examples/nsl_pk/DY.Example.NSL.Protocol.Total.Proof.fst
@@ -28,17 +28,17 @@ let crypto_predicates_nsl = {
         | Some (Msg1 msg1) -> (
           let (alice, bob) = (msg1.alice, prin) in
           event_triggered tr alice (Initiate1 alice bob msg1.n_a) /\
-          get_label tr msg1.n_a == join (principal_label alice) (principal_label bob)
+          get_label tr msg1.n_a == join (nsl_nonce_label alice) (nsl_nonce_label bob)
         )
         | Some (Msg2 msg2) -> (
           let (alice, bob) = (prin, msg2.bob) in
           event_triggered tr bob (Respond1 alice bob msg2.n_a msg2.n_b) /\
-          get_label tr msg2.n_b == join (principal_label alice) (principal_label bob)
+          get_label tr msg2.n_b == join (nsl_nonce_label alice) (nsl_nonce_label bob)
         )
         | Some (Msg3 msg3) -> (
           let bob = prin in
           exists alice n_a.
-            get_label tr msg3.n_b `can_flow tr` (principal_label alice) /\
+            get_label tr msg3.n_b `can_flow tr` (nsl_nonce_label alice) /\
             event_triggered tr alice (Initiate2 alice bob n_a msg3.n_b)
         )
         | None -> False
@@ -66,9 +66,9 @@ val compute_message1_proof:
     // From the stateful code
     event_triggered tr alice (Initiate1 alice bob n_a) /\
     // From random generation
-    is_secret (join (principal_label alice) (principal_label bob)) tr n_a  /\
+    is_secret (join (nsl_nonce_label alice) (nsl_nonce_label bob)) tr n_a  /\
     // From random generation
-    is_secret (principal_label alice) tr nonce /\
+    is_secret (long_term_key_label alice) tr nonce /\
     // From random generation
     PkNonce? (get_usage nonce) /\
     // From PKI invariants
@@ -77,8 +77,10 @@ val compute_message1_proof:
   (ensures is_publishable tr (compute_message1 alice bob pk_b n_a nonce))
 let compute_message1_proof tr alice bob pk_b n_a nonce =
   let msg = Msg1 {n_a; alice;} in
-  serialize_wf_lemma message (is_knowable_by (principal_label alice) tr) msg;
-  serialize_wf_lemma message (is_knowable_by (principal_label bob) tr) msg
+  assert(join (nsl_nonce_label alice) (nsl_nonce_label bob) `can_flow tr` (nsl_nonce_label alice));
+  assert(join (nsl_nonce_label alice) (nsl_nonce_label bob) `can_flow tr` (nsl_nonce_label bob));
+  serialize_wf_lemma message (is_knowable_by (long_term_key_label alice) tr) msg;
+  serialize_wf_lemma message (is_knowable_by (long_term_key_label bob) tr) msg
 
 // If bob successfully decrypt the first message,
 // then n_a is knownable both by alice (in the message) and bob (the principal)
@@ -100,7 +102,7 @@ val decode_message1_proof:
     match decode_message1 bob msg_cipher sk_b with
     | None -> True
     | Some msg1 -> (
-      is_knowable_by (join (principal_label msg1.alice) (principal_label bob)) tr msg1.n_a
+      is_knowable_by (join (nsl_nonce_label msg1.alice) (nsl_nonce_label bob)) tr msg1.n_a
     )
   ))
 let decode_message1_proof tr bob msg_cipher sk_b =
@@ -120,11 +122,11 @@ val compute_message2_proof:
     // From the stateful code
     event_triggered tr bob (Respond1 msg1.alice bob msg1.n_a n_b) /\
     // From decode_message1_proof
-    is_knowable_by (join (principal_label msg1.alice) (principal_label bob)) tr msg1.n_a /\
+    is_knowable_by (join (nsl_nonce_label msg1.alice) (nsl_nonce_label bob)) tr msg1.n_a /\
     // From the random generation
-    is_secret (join (principal_label msg1.alice) (principal_label bob)) tr n_b /\
+    is_secret (join (nsl_nonce_label msg1.alice) (nsl_nonce_label bob)) tr n_b /\
     // From the random generation
-    is_secret (principal_label bob) tr nonce /\
+    is_secret (long_term_key_label bob) tr nonce /\
     // From the random generation
     PkNonce? (get_usage nonce) /\
     // From the PKI
@@ -135,8 +137,8 @@ val compute_message2_proof:
   )
 let compute_message2_proof tr bob msg1 pk_a n_b nonce =
   let msg = Msg2 {n_a = msg1.n_a;  n_b; bob;} in
-  serialize_wf_lemma message (is_knowable_by (principal_label msg1.alice) tr) msg;
-  serialize_wf_lemma message (is_knowable_by (principal_label bob) tr) msg
+  serialize_wf_lemma message (is_knowable_by (nsl_nonce_label msg1.alice) tr) msg;
+  serialize_wf_lemma message (is_knowable_by (nsl_nonce_label bob) tr) msg
 
 // If alice successfully decrypt the second message,
 // then n_b is knownable both by alice (in the message) and bob (the principal)
@@ -150,7 +152,7 @@ val decode_message2_proof:
   Lemma
   (requires
     // From the NSL state invariant
-    is_secret (join (principal_label alice) (principal_label bob)) tr n_a /\
+    is_secret (join (nsl_nonce_label alice) (nsl_nonce_label bob)) tr n_a /\
     // From the PrivateKeys invariant
     is_private_key_for tr sk_a (LongTermPkEncKey "NSL.PublicKey") alice /\
     // From the network
@@ -160,8 +162,8 @@ val decode_message2_proof:
     match decode_message2 alice bob msg_cipher sk_a n_a with
     | None -> True
     | Some msg2 -> (
-      is_knowable_by (join (principal_label alice) (principal_label bob)) tr msg2.n_b /\ (
-      (is_corrupt tr (principal_label alice) \/ is_corrupt tr (principal_label bob)) \/ (
+      is_knowable_by (join (nsl_nonce_label alice) (nsl_nonce_label bob)) tr msg2.n_b /\ (
+      (is_corrupt tr (nsl_nonce_label alice) \/ is_corrupt tr (nsl_nonce_label bob)) \/ (
         event_triggered tr bob (Respond1 alice bob n_a msg2.n_b)
       )
       )
@@ -185,9 +187,9 @@ val compute_message3_proof:
     // From the stateful code
     (exists n_a. event_triggered tr alice (Initiate2 alice bob n_a n_b)) /\
     // From decode_message2_proof
-    is_knowable_by (join (principal_label alice) (principal_label bob)) tr n_b /\
+    is_knowable_by (join (nsl_nonce_label alice) (nsl_nonce_label bob)) tr n_b /\
     // From the random generation
-    is_secret (principal_label alice) tr nonce /\
+    is_secret (long_term_key_label alice) tr nonce /\
     // From the random generation
     PkNonce? (get_usage nonce) /\
     // From the PKI
@@ -199,8 +201,8 @@ val compute_message3_proof:
 let compute_message3_proof tr alice bob pk_b n_b nonce =
   assert(exists alice n_a. event_triggered tr alice (Initiate2 alice bob n_a n_b));
   let msg = Msg3 {n_b;} in
-  serialize_wf_lemma message (is_knowable_by (principal_label alice) tr) msg;
-  serialize_wf_lemma message (is_knowable_by (principal_label bob) tr) msg;
+  serialize_wf_lemma message (is_knowable_by (long_term_key_label alice) tr) msg;
+  serialize_wf_lemma message (is_knowable_by (long_term_key_label bob) tr) msg;
   let msg3: message3 = {n_b;} in
   assert(msg3.n_b == n_b)
 
@@ -214,7 +216,7 @@ val decode_message3_proof:
   Lemma
   (requires
     // From the NSL state invariant
-    get_label tr n_b == join (principal_label alice) (principal_label bob) /\
+    get_label tr n_b == join (nsl_nonce_label alice) (nsl_nonce_label bob) /\
     // From the PrivateKeys invariant
     is_private_key_for tr sk_b (LongTermPkEncKey "NSL.PublicKey") bob /\
     // From the network
@@ -224,9 +226,9 @@ val decode_message3_proof:
     match decode_message3 alice bob msg_cipher sk_b n_b with
     | None -> True
     | Some msg3 -> (
-      (is_corrupt tr (principal_label alice) \/ is_corrupt tr (principal_label bob)) \/ (
+      (is_corrupt tr (nsl_nonce_label alice) \/ is_corrupt tr (nsl_nonce_label bob)) \/ (
         (exists alice n_a.
-          get_label tr msg3.n_b `can_flow tr` (principal_label alice) /\
+          get_label tr msg3.n_b `can_flow tr` (nsl_nonce_label alice) /\
           event_triggered tr alice (Initiate2 alice bob n_a n_b))
       )
     )
